_:B69151a89349678f3f9ee83d0310425b8 <http://www.w3.org/1999/02/22-rdf-syntax-ns#rest> _:B3aca6c79836c36ea955880b81ce5ed9d .
_:B69151a89349678f3f9ee83d0310425b8 <http://www.w3.org/1999/02/22-rdf-syntax-ns#first> <http://www.ondex.org/bioknet/terms/Accession> .
<http://www.ondex.org/bioknet/terms/relTypeRef> <http://www.w3.org/2000/01/rdf-schema#domain> <http://www.ondex.org/bioknet/terms/Relation> .
<http://www.ondex.org/bioknet/terms/relTypeRef> <http://www.w3.org/2004/02/skos/core#editorialNote> "The fact that the values of this should be subclasses of bk:relationType is documented by means of schema:rangeIncludes. We don't use rdfs:range bk:relationType, because this tends to confuse ontology editors and libraries (i.e., Protege and OWL-API), which infer bk:relationType is also a clsass. It shouldn't be a big deal to link to bk:relationType using an owl:objectProperty like this, since OWL-2 should deal with this through punning (TODO: check)."@en .
<http://www.ondex.org/bioknet/terms/relTypeRef> <http://www.w3.org/2000/01/rdf-schema#comment> "[editorial note] The fact that the values of this should be subclasses of bk:relationType is documented by means of schema:rangeIncludes. We don't use rdfs:range bk:relationType, because this tends to confuse ontology editors and libraries (i.e., Protege and OWL-API), which infer bk:relationType is also a clsass. It shouldn't be a big deal to link to bk:relationType using an owl:objectProperty like this, since OWL-2 should deal with this through punning (TODO: check)." .
<http://www.ondex.org/bioknet/terms/relTypeRef> <http://www.w3.org/1999/02/22-rdf-syntax-ns#type> <http://www.w3.org/2002/07/owl#ObjectProperty> .
<http://www.ondex.org/bioknet/terms/relTypeRef> <https://schema.org/rangeIncludes> <http://www.ondex.org/bioknet/terms/relationType> .
<http://www.ondex.org/bioknet/terms/relTypeRef> <http://www.w3.org/2000/01/rdf-schema#label> "is instance of relation type"@en .
<http://www.ondex.org/bioknet/terms/DataSource> <http://www.w3.org/2000/01/rdf-schema#subClassOf> <http://www.ondex.org/bioknet/terms/Describeable> .
<http://www.ondex.org/bioknet/terms/DataSource> <http://www.w3.org/1999/02/22-rdf-syntax-ns#type> <http://www.w3.org/2002/07/owl#Class> .
<http://www.ondex.org/bioknet/terms/DataSource> <http://www.w3.org/2000/01/rdf-schema#label> "Data Source"@en .
<http://www.ondex.org/bioknet/terms/attributeValue> <http://www.w3.org/2000/01/rdf-schema#domain> <http://www.ondex.org/bioknet/terms/Attribute> .
<http://www.ondex.org/bioknet/terms/attributeValue> <http://www.w3.org/1999/02/22-rdf-syntax-ns#type> <http://www.w3.org/2002/07/owl#DatatypeProperty> .
<http://www.ondex.org/bioknet/terms/attributeValue> <http://www.w3.org/2000/01/rdf-schema#label> "attribute value"@en .
<http://www.ondex.org/bioknet/terms/relTo> <http://www.w3.org/2000/01/rdf-schema#domain> <http://www.ondex.org/bioknet/terms/Relation> .
<http://www.ondex.org/bioknet/terms/relTo> <http://www.w3.org/1999/02/22-rdf-syntax-ns#type> <http://www.w3.org/2002/07/owl#ObjectProperty> .
<http://www.ondex.org/bioknet/terms/relTo> <http://www.w3.org/2000/01/rdf-schema#range> <http://www.ondex.org/bioknet/terms/Concept> .
<http://www.ondex.org/bioknet/terms/Concept> <http://www.w3.org/2004/02/skos/core#editorialNote> "Those used to the ONDEX model should note that we are mapping the conceptType relations straight to rdf:type and the ONDEX Concept Classes to rdfs:subClassOf this class. We see this as a natural mapping of the ONDEX model to the RDF/RDF-S/OWL standards."@en .
<http://www.ondex.org/bioknet/terms/Concept> <http://www.w3.org/2000/01/rdf-schema#comment> "[editorial note] Those used to the ONDEX model should note that we are mapping the conceptType relations straight to rdf:type and the ONDEX Concept Classes to rdfs:subClassOf this class. We see this as a natural mapping of the ONDEX model to the RDF/RDF-S/OWL standards." .
<http://www.ondex.org/bioknet/terms/Concept> <http://www.w3.org/2000/01/rdf-schema#comment> "[description] A Concept is the a basic unit of information in the Bio Knowledge Network Ontology. The main type of knowledge in BioKNet consists of relations (either RDF triples based on bk:relationType, or bk:Relation instances) between bk:Concept instances.\n\nThe recommended way to use bk:Concept and bk:ConceptClass is: \n  - subclass bk:ConceptClass with specific classes (eg, Protein, Gene)\n  - instance those specific classes\n  - optionally, but recommended in production environment like triple stores backing SPARQL, declare your new instance an instance of bk:Concept too. While this can be inferred, having explicit instances make things easier for applications.\n\nNote also that bk:Concept should never be subclassed with specific network classes, use bk:ConceptClass instead." .
<http://www.ondex.org/bioknet/terms/Concept> <http://www.w3.org/2000/01/rdf-schema#subClassOf> <http://www.ondex.org/bioknet/terms/RelationElement> .
<http://www.ondex.org/bioknet/terms/Concept> <http://www.w3.org/1999/02/22-rdf-syntax-ns#type> <http://www.w3.org/2002/07/owl#Class> .
<http://www.ondex.org/bioknet/terms/Concept> <http://purl.org/dc/terms/description> "A Concept is the a basic unit of information in the Bio Knowledge Network Ontology. The main type of knowledge in BioKNet consists of relations (either RDF triples based on bk:relationType, or bk:Relation instances) between bk:Concept instances.\n\nThe recommended way to use bk:Concept and bk:ConceptClass is: \n  - subclass bk:ConceptClass with specific classes (eg, Protein, Gene)\n  - instance those specific classes\n  - optionally, but recommended in production environment like triple stores backing SPARQL, declare your new instance an instance of bk:Concept too. While this can be inferred, having explicit instances make things easier for applications.\n\nNote also that bk:Concept should never be subclassed with specific network classes, use bk:ConceptClass instead."@en .
<http://www.ondex.org/bioknet/terms/Concept> <http://www.w3.org/2000/01/rdf-schema#label> "Concept"@en .
<http://www.ondex.org/bioknet/terms/> <http://www.w3.org/1999/02/22-rdf-syntax-ns#type> <http://www.w3.org/2002/07/owl#Ontology> .
<http://www.ondex.org/bioknet/terms/isAmbiguousAccession> <http://www.w3.org/2000/01/rdf-schema#domain> <http://www.ondex.org/bioknet/terms/Accession> .
<http://www.ondex.org/bioknet/terms/isAmbiguousAccession> <http://www.w3.org/2004/02/skos/core#editorialNote> "TODO: we need to clarify what this is exactly. How can an accession be ambiguous? Examples?"@en .
<http://www.ondex.org/bioknet/terms/isAmbiguousAccession> <http://www.w3.org/2000/01/rdf-schema#comment> "[editorial note] TODO: we need to clarify what this is exactly. How can an accession be ambiguous? Examples?" .
<http://www.ondex.org/bioknet/terms/isAmbiguousAccession> <http://www.w3.org/1999/02/22-rdf-syntax-ns#type> <http://www.w3.org/2002/07/owl#DatatypeProperty> .
<http://www.ondex.org/bioknet/terms/isAmbiguousAccession> <http://www.w3.org/2000/01/rdf-schema#range> <http://www.w3.org/2001/XMLSchema#boolean> .
<http://www.ondex.org/bioknet/terms/isAmbiguousAccession> <http://www.w3.org/2000/01/rdf-schema#label> "is ambiguous accession"@en .
<http://www.ondex.org/bioknet/terms/testProp> <http://www.w3.org/2000/01/rdf-schema#subPropertyOf> <http://www.ondex.org/bioknet/terms/relationType> .
<http://www.ondex.org/bioknet/terms/testProp> <http://www.w3.org/2000/01/rdf-schema#comment> "[description] Just a test relation." .
<http://www.ondex.org/bioknet/terms/testProp> <http://www.w3.org/1999/02/22-rdf-syntax-ns#type> <http://www.w3.org/2002/07/owl#NamedIndividual> .
<http://www.ondex.org/bioknet/terms/testProp> <http://www.w3.org/1999/02/22-rdf-syntax-ns#type> <http://www.w3.org/2002/07/owl#ObjectProperty> .
<http://www.ondex.org/bioknet/terms/testProp> <http://purl.org/dc/terms/description> "Just a test relation."@en .
<http://www.w3.org/2004/02/skos/core#editorialNote> <http://www.w3.org/1999/02/22-rdf-syntax-ns#type> <http://www.w3.org/2002/07/owl#AnnotationProperty> .
<http://www.ondex.org/bioknet/terms/testStmt0> <http://www.ondex.org/bioknet/terms/relTypeRef> <http://www.ondex.org/bioknet/terms/testProp> .
<http://www.ondex.org/bioknet/terms/testStmt0> <http://www.w3.org/1999/02/22-rdf-syntax-ns#type> <http://www.w3.org/2002/07/owl#NamedIndividual> .
<http://www.ondex.org/bioknet/terms/testStmt0> <http://www.w3.org/1999/02/22-rdf-syntax-ns#type> <http://www.ondex.org/bioknet/terms/Relation> .
<http://www.ondex.org/bioknet/terms/graphConceptsCount> <http://www.w3.org/2000/01/rdf-schema#subPropertyOf> <http://www.ondex.org/bioknet/terms/graphSummaryFigure> .
<http://www.ondex.org/bioknet/terms/graphConceptsCount> <http://www.w3.org/1999/02/22-rdf-syntax-ns#type> <http://www.w3.org/2002/07/owl#DatatypeProperty> .
<http://www.ondex.org/bioknet/terms/graphConceptsCount> <http://www.w3.org/2000/01/rdf-schema#range> <http://www.w3.org/2001/XMLSchema#long> .
<http://www.ondex.org/bioknet/terms/graphConceptsCount> <http://www.w3.org/2000/01/rdf-schema#label> "graph concepts count"@en .
<http://www.ondex.org/bioknet/terms/RelationElement> <http://www.w3.org/2000/01/rdf-schema#comment> "[description] A bk:Relation, or the corresponding BioKNet triple, is composed mainly of two bk:Concept instances and a relation type. The bk:RelationElement is a convenience common container for such components." .
<http://www.ondex.org/bioknet/terms/RelationElement> <http://www.w3.org/2000/01/rdf-schema#seeAlso> <http://www.ondex.org/bioknet/terms/Concept> .
<http://www.ondex.org/bioknet/terms/RelationElement> <http://www.w3.org/2000/01/rdf-schema#seeAlso> <http://www.ondex.org/bioknet/terms/Relation> .
<http://www.ondex.org/bioknet/terms/RelationElement> <http://www.w3.org/1999/02/22-rdf-syntax-ns#type> <http://www.w3.org/2002/07/owl#Class> .
<http://www.ondex.org/bioknet/terms/RelationElement> <http://purl.org/dc/terms/description> "A bk:Relation, or the corresponding BioKNet triple, is composed mainly of two bk:Concept instances and a relation type. The bk:RelationElement is a convenience common container for such components."@en .
<http://www.ondex.org/bioknet/terms/RelationElement> <http://www.w3.org/2000/01/rdf-schema#label> "Relation Element"@en .
<http://www.ondex.org/bioknet/terms/attributeTypeUnit> <http://www.w3.org/2000/01/rdf-schema#domain> <http://www.ondex.org/bioknet/terms/AttributeType> .
<http://www.ondex.org/bioknet/terms/attributeTypeUnit> <http://www.w3.org/1999/02/22-rdf-syntax-ns#type> <http://www.w3.org/2002/07/owl#ObjectProperty> .
<http://www.ondex.org/bioknet/terms/attributeTypeUnit> <http://www.w3.org/2000/01/rdf-schema#range> <http://www.ondex.org/bioknet/terms/Unit> .
<http://www.ondex.org/bioknet/terms/relFrom> <http://www.w3.org/2000/01/rdf-schema#domain> <http://www.ondex.org/bioknet/terms/Relation> .
<http://www.ondex.org/bioknet/terms/relFrom> <http://www.w3.org/1999/02/22-rdf-syntax-ns#type> <http://www.w3.org/2002/07/owl#ObjectProperty> .
<http://www.ondex.org/bioknet/terms/relFrom> <http://www.w3.org/2000/01/rdf-schema#range> <http://www.ondex.org/bioknet/terms/Concept> .
_:Beba9e75bdb592ddd3419c296663ececd <http://www.w3.org/2002/07/owl#onProperty> <http://www.ondex.org/bioknet/terms/dataSource> .
_:Beba9e75bdb592ddd3419c296663ececd <http://www.w3.org/1999/02/22-rdf-syntax-ns#type> <http://www.w3.org/2002/07/owl#Restriction> .
_:Beba9e75bdb592ddd3419c296663ececd <http://www.w3.org/2002/07/owl#someValuesFrom> <http://www.ondex.org/bioknet/terms/DataSource> .
<http://www.ondex.org/bioknet/terms/attribute> <http://www.w3.org/2000/01/rdf-schema#domain> <http://www.ondex.org/bioknet/terms/RelationElement> .
<http://www.ondex.org/bioknet/terms/attribute> <http://www.w3.org/1999/02/22-rdf-syntax-ns#type> <http://www.w3.org/2002/07/owl#ObjectProperty> .
<http://www.ondex.org/bioknet/terms/attribute> <http://www.w3.org/2000/01/rdf-schema#range> <http://www.ondex.org/bioknet/terms/Attribute> .
<http://www.ondex.org/bioknet/terms/graphSummaryFigure> <http://www.w3.org/2000/01/rdf-schema#domain> <http://www.ondex.org/bioknet/terms/Graph> .
<http://www.ondex.org/bioknet/terms/graphSummaryFigure> <http://www.w3.org/2000/01/rdf-schema#comment> "[description] a property of this type provides summary figures for the contents of a graph, such as the number of concepts or relations." .
<http://www.ondex.org/bioknet/terms/graphSummaryFigure> <http://www.w3.org/1999/02/22-rdf-syntax-ns#type> <http://www.w3.org/2002/07/owl#DatatypeProperty> .
<http://www.ondex.org/bioknet/terms/graphSummaryFigure> <http://purl.org/dc/terms/description> "a property of this type provides summary figures for the contents of a graph, such as the number of concepts or relations."@en .
<http://www.ondex.org/bioknet/terms/graphSummaryFigure> <http://www.w3.org/2000/01/rdf-schema#label> "graph summary figure"@en .
<http://www.ondex.org/bioknet/terms/evidence> <http://www.w3.org/2000/01/rdf-schema#domain> <http://www.ondex.org/bioknet/terms/RelationElement> .
<http://www.ondex.org/bioknet/terms/evidence> <http://www.w3.org/2000/01/rdf-schema#comment> "[description] Links an entity, such as a concept or a relation, to the type of evidence that prove it exists, such as 'imported from database', evidence codes, 'inferred from literature'." .
<http://www.ondex.org/bioknet/terms/evidence> <http://www.w3.org/1999/02/22-rdf-syntax-ns#type> <http://www.w3.org/2002/07/owl#ObjectProperty> .
<http://www.ondex.org/bioknet/terms/evidence> <http://www.w3.org/2000/01/rdf-schema#range> <http://www.ondex.org/bioknet/terms/EvidenceType> .
<http://www.ondex.org/bioknet/terms/evidence> <http://purl.org/dc/terms/description> "Links an entity, such as a concept or a relation, to the type of evidence that prove it exists, such as 'imported from database', evidence codes, 'inferred from literature'."@en .
_:B893e6b0794adfa99a28a8941ce54d52f <http://www.w3.org/2002/07/owl#onClass> <http://www.ondex.org/bioknet/terms/AttributeType> .
_:B893e6b0794adfa99a28a8941ce54d52f <http://www.w3.org/2002/07/owl#onProperty> <http://www.ondex.org/bioknet/terms/attributeType> .
_:B893e6b0794adfa99a28a8941ce54d52f <http://www.w3.org/2002/07/owl#qualifiedCardinality> "1"^^<http://www.w3.org/2001/XMLSchema#nonNegativeInteger> .
_:B893e6b0794adfa99a28a8941ce54d52f <http://www.w3.org/1999/02/22-rdf-syntax-ns#type> <http://www.w3.org/2002/07/owl#Restriction> .
<http://www.ondex.org/bioknet/terms/relationType> <http://www.w3.org/2000/01/rdf-schema#domain> <http://www.ondex.org/bioknet/terms/Concept> .
<http://www.ondex.org/bioknet/terms/relationType> <http://www.w3.org/2000/01/rdf-schema#comment> "[description] This is a top-level placeholder for relevant knowledge relations between bk:Concept instances. See bk:Relation for a detailed description of how relations are model in BioKNet," .
<http://www.ondex.org/bioknet/terms/relationType> <http://www.w3.org/2000/01/rdf-schema#seeAlso> <http://www.ondex.org/bioknet/terms/Relation> .
<http://www.ondex.org/bioknet/terms/relationType> <http://www.w3.org/1999/02/22-rdf-syntax-ns#type> <http://www.w3.org/2002/07/owl#ObjectProperty> .
<http://www.ondex.org/bioknet/terms/relationType> <http://www.w3.org/2000/01/rdf-schema#range> <http://www.ondex.org/bioknet/terms/Concept> .
<http://www.ondex.org/bioknet/terms/relationType> <http://purl.org/dc/terms/description> "This is a top-level placeholder for relevant knowledge relations between bk:Concept instances. See bk:Relation for a detailed description of how relations are model in BioKNet,"@en .
<http://www.ondex.org/bioknet/terms/relationType> <http://www.w3.org/2000/01/rdf-schema#label> "is related to"@en .
<http://www.ondex.org/bioknet/terms/AttributeType> <http://www.w3.org/2004/02/skos/core#editorialNote> "This is AttributeName in ONDEX. It doesn't look correct to call it name."@en .
<http://www.ondex.org/bioknet/terms/AttributeType> <http://www.w3.org/2000/01/rdf-schema#comment> "[editorial note] This is AttributeName in ONDEX. It doesn't look correct to call it name." .
<http://www.ondex.org/bioknet/terms/AttributeType> <http://www.w3.org/2000/01/rdf-schema#subClassOf> _:B77861368e8bb2f8d2dfef6b68718e585 .
<http://www.ondex.org/bioknet/terms/AttributeType> <http://www.w3.org/2000/01/rdf-schema#subClassOf> <http://www.ondex.org/bioknet/terms/Describeable> .
<http://www.ondex.org/bioknet/terms/AttributeType> <http://www.w3.org/1999/02/22-rdf-syntax-ns#type> <http://www.w3.org/2002/07/owl#Class> .
<http://www.ondex.org/bioknet/terms/AttributeType> <http://www.w3.org/2000/01/rdf-schema#label> "Attribute Type"@en .
<http://www.ondex.org/bioknet/terms/ConceptClass> <http://www.w3.org/2000/01/rdf-schema#comment> "[description] bk:ConceptClass is a convenience container to be used to subclass bk:Concept. Application-specific concept types should be subclassed starting from here." .
<http://www.ondex.org/bioknet/terms/ConceptClass> <http://www.w3.org/2000/01/rdf-schema#seeAlso> <http://www.ondex.org/bioknet/terms/Concept> .
<http://www.ondex.org/bioknet/terms/ConceptClass> <http://www.w3.org/2000/01/rdf-schema#seeAlso> <http://www.ondex.org/bioknet/terms/Relation> .
<http://www.ondex.org/bioknet/terms/ConceptClass> <http://www.w3.org/2000/01/rdf-schema#subClassOf> <http://www.ondex.org/bioknet/terms/Concept> .
<http://www.ondex.org/bioknet/terms/ConceptClass> <http://www.w3.org/2000/01/rdf-schema#subClassOf> <http://www.ondex.org/bioknet/terms/Describeable> .
<http://www.ondex.org/bioknet/terms/ConceptClass> <http://www.w3.org/1999/02/22-rdf-syntax-ns#type> <http://www.w3.org/2002/07/owl#Class> .
<http://www.ondex.org/bioknet/terms/ConceptClass> <http://purl.org/dc/terms/description> "bk:ConceptClass is a convenience container to be used to subclass bk:Concept. Application-specific concept types should be subclassed starting from here."@en .
<http://www.ondex.org/bioknet/terms/ConceptClass> <http://www.w3.org/2000/01/rdf-schema#label> "Concept Class"@en .
<http://www.ondex.org/bioknet/terms/attributeType> <http://www.w3.org/2000/01/rdf-schema#domain> <http://www.ondex.org/bioknet/terms/Attribute> .
<http://www.ondex.org/bioknet/terms/attributeType> <http://www.w3.org/1999/02/22-rdf-syntax-ns#type> <http://www.w3.org/2002/07/owl#ObjectProperty> .
<http://www.ondex.org/bioknet/terms/attributeType> <http://www.w3.org/2000/01/rdf-schema#range> <http://www.ondex.org/bioknet/terms/AttributeType> .
<http://www.ondex.org/bioknet/terms/graphRelationsCount> <http://www.w3.org/2000/01/rdf-schema#subPropertyOf> <http://www.ondex.org/bioknet/terms/graphSummaryFigure> .
<http://www.ondex.org/bioknet/terms/graphRelationsCount> <http://www.w3.org/1999/02/22-rdf-syntax-ns#type> <http://www.w3.org/2002/07/owl#DatatypeProperty> .
<http://www.ondex.org/bioknet/terms/graphRelationsCount> <http://www.w3.org/2000/01/rdf-schema#range> <http://www.w3.org/2001/XMLSchema#long> .
<http://www.ondex.org/bioknet/terms/graphRelationsCount> <http://www.w3.org/2000/01/rdf-schema#label> "graph relations count"@en .
<http://www.ondex.org/bioknet/terms/name> <http://www.w3.org/2004/02/skos/core#editorialNote> "Compared to the ONDEX model, we use bk:prefName to represent a name that has the preferred flag set to true, bk:altName to represent all the other names, bk:name for generic names. This is simpler than having a class just to store an additional flag."@en .
<http://www.ondex.org/bioknet/terms/name> <http://www.w3.org/2000/01/rdf-schema#comment> "[editorial note] Compared to the ONDEX model, we use bk:prefName to represent a name that has the preferred flag set to true, bk:altName to represent all the other names, bk:name for generic names. This is simpler than having a class just to store an additional flag." .
<http://www.ondex.org/bioknet/terms/name> <http://www.w3.org/2000/01/rdf-schema#comment> "[description] In bio-databases a name is often meant as something more specific than a title or a label (being more official and often shorter) and not as unique as accessions." .
<http://www.ondex.org/bioknet/terms/name> <http://www.w3.org/1999/02/22-rdf-syntax-ns#type> <http://www.w3.org/2002/07/owl#DatatypeProperty> .
<http://www.ondex.org/bioknet/terms/name> <http://www.w3.org/2000/01/rdf-schema#range> <http://www.w3.org/2001/XMLSchema#string> .
<http://www.ondex.org/bioknet/terms/name> <http://purl.org/dc/terms/description> "In bio-databases a name is often meant as something more specific than a title or a label (being more official and often shorter) and not as unique as accessions."@en .
<http://www.ondex.org/bioknet/terms/name> <http://www.w3.org/2000/01/rdf-schema#label> "has name"@en .
<http://www.ondex.org/bioknet/terms/Graph> <http://www.w3.org/2004/02/skos/core#editorialNote> "[TODO] to be completed, using VoID, pav, etc."@en .
<http://www.ondex.org/bioknet/terms/Graph> <http://www.w3.org/2000/01/rdf-schema#comment> "[editorial note] [TODO] to be completed, using VoID, pav, etc." .
<http://www.ondex.org/bioknet/terms/Graph> <http://www.w3.org/2000/01/rdf-schema#comment> "[description] A biological knowledge network can be grouped together into a graph. This is typically a named graph as well and used in triple stores like Virtuoso to identify networks/subsets." .
<http://www.ondex.org/bioknet/terms/Graph> <http://www.w3.org/1999/02/22-rdf-syntax-ns#type> <http://www.w3.org/2002/07/owl#Class> .
<http://www.ondex.org/bioknet/terms/Graph> <http://purl.org/dc/terms/description> "A biological knowledge network can be grouped together into a graph. This is typically a named graph as well and used in triple stores like Virtuoso to identify networks/subsets."@en .
<http://www.ondex.org/bioknet/terms/Graph> <http://www.w3.org/2000/01/rdf-schema#label> "Graph"@en .
<http://www.ondex.org/bioknet/terms/Attribute> <http://www.w3.org/2004/02/skos/core#editorialNote> "Note that this is different than other structured value models (e.g., schema.org, good relations), where units can be specified for each value. Here these are linked to the type for all the values of that type."@en .
<http://www.ondex.org/bioknet/terms/Attribute> <http://www.w3.org/2000/01/rdf-schema#comment> "[editorial note] Note that this is different than other structured value models (e.g., schema.org, good relations), where units can be specified for each value. Here these are linked to the type for all the values of that type." .
<http://www.ondex.org/bioknet/terms/Attribute> <http://www.w3.org/2000/01/rdf-schema#comment> "[description] An attribute is a literal value associated to a type. The type might optionally tell a unit for the literal value (presumably a number)." .
<http://www.ondex.org/bioknet/terms/Attribute> <http://www.w3.org/2000/01/rdf-schema#subClassOf> _:B893e6b0794adfa99a28a8941ce54d52f .
<http://www.ondex.org/bioknet/terms/Attribute> <http://www.w3.org/2000/01/rdf-schema#subClassOf> _:Bd02e7d92de08425eedaa31399e7ae755 .
<http://www.ondex.org/bioknet/terms/Attribute> <http://www.w3.org/1999/02/22-rdf-syntax-ns#type> <http://www.w3.org/2002/07/owl#Class> .
<http://www.ondex.org/bioknet/terms/Attribute> <http://purl.org/dc/terms/description> "An attribute is a literal value associated to a type. The type might optionally tell a unit for the literal value (presumably a number)."@en .
<http://www.ondex.org/bioknet/terms/Attribute> <http://www.w3.org/2000/01/rdf-schema#label> "Attribute"@en .
<http://www.ondex.org/bioknet/terms/prefName> <http://www.w3.org/2000/01/rdf-schema#subPropertyOf> <http://www.ondex.org/bioknet/terms/name> .
<http://www.ondex.org/bioknet/terms/prefName> <http://www.w3.org/1999/02/22-rdf-syntax-ns#type> <http://www.w3.org/2002/07/owl#DatatypeProperty> .
<http://www.ondex.org/bioknet/terms/prefName> <http://www.w3.org/2000/01/rdf-schema#label> "has preferred name"@en .
<http://www.ondex.org/bioknet/terms/dataSource> <http://www.w3.org/2000/01/rdf-schema#domain> _:Bec150e6e8653b51fcd8e13b7cab86016 .
<http://www.ondex.org/bioknet/terms/dataSource> <http://www.w3.org/2004/02/skos/core#editorialNote> "[TODO] Align to PAV and alike."@en .
<http://www.ondex.org/bioknet/terms/dataSource> <http://www.w3.org/2000/01/rdf-schema#comment> "[editorial note] [TODO] Align to PAV and alike." .
<http://www.ondex.org/bioknet/terms/dataSource> <http://www.w3.org/2000/01/rdf-schema#comment> "[description] The source from which an entity comes from, or was imported or alike." .
<http://www.ondex.org/bioknet/terms/dataSource> <http://www.w3.org/1999/02/22-rdf-syntax-ns#type> <http://www.w3.org/2002/07/owl#ObjectProperty> .
<http://www.ondex.org/bioknet/terms/dataSource> <http://www.w3.org/2000/01/rdf-schema#range> <http://www.ondex.org/bioknet/terms/DataSource> .
<http://www.ondex.org/bioknet/terms/dataSource> <http://purl.org/dc/terms/description> "The source from which an entity comes from, or was imported or alike."@en .
_:Bd02e7d92de08425eedaa31399e7ae755 <http://www.w3.org/2002/07/owl#onProperty> <http://www.ondex.org/bioknet/terms/attributeValue> .
_:Bd02e7d92de08425eedaa31399e7ae755 <http://www.w3.org/1999/02/22-rdf-syntax-ns#type> <http://www.w3.org/2002/07/owl#Restriction> .
_:Bd02e7d92de08425eedaa31399e7ae755 <http://www.w3.org/2002/07/owl#cardinality> "1"^^<http://www.w3.org/2001/XMLSchema#nonNegativeInteger> .
<http://www.ondex.org/bioknet/terms/Accession> <http://www.w3.org/2000/01/rdf-schema#comment> "[description] An accession is a string value, assigned with dcterms:identifier and at least one data source in which the accession value is usually unique. Set bk:isAccessionAmbiguous to false to specify the accession is not necessarily unique." .
<http://www.ondex.org/bioknet/terms/Accession> <http://www.w3.org/2000/01/rdf-schema#subClassOf> _:Beba9e75bdb592ddd3419c296663ececd .
<http://www.ondex.org/bioknet/terms/Accession> <http://www.w3.org/1999/02/22-rdf-syntax-ns#type> <http://www.w3.org/2002/07/owl#Class> .
<http://www.ondex.org/bioknet/terms/Accession> <http://purl.org/dc/terms/description> "An accession is a string value, assigned with dcterms:identifier and at least one data source in which the accession value is usually unique. Set bk:isAccessionAmbiguous to false to specify the accession is not necessarily unique."@en .
<http://www.ondex.org/bioknet/terms/Accession> <http://www.w3.org/2000/01/rdf-schema#label> "Accession"@en .
<http://www.ondex.org/bioknet/terms/altName> <http://www.w3.org/2000/01/rdf-schema#subPropertyOf> <http://www.ondex.org/bioknet/terms/name> .
<http://www.ondex.org/bioknet/terms/altName> <http://www.w3.org/1999/02/22-rdf-syntax-ns#type> <http://www.w3.org/2002/07/owl#DatatypeProperty> .
<http://www.ondex.org/bioknet/terms/altName> <http://www.w3.org/2000/01/rdf-schema#label> "has alternative name"@en .
_:B3aca6c79836c36ea955880b81ce5ed9d <http://www.w3.org/1999/02/22-rdf-syntax-ns#rest> <http://www.w3.org/1999/02/22-rdf-syntax-ns#nil> .
_:B3aca6c79836c36ea955880b81ce5ed9d <http://www.w3.org/1999/02/22-rdf-syntax-ns#first> <http://www.ondex.org/bioknet/terms/RelationElement> .
<http://www.ondex.org/bioknet/terms/Unit> <http://www.w3.org/2000/01/rdf-schema#subClassOf> <http://www.ondex.org/bioknet/terms/Describeable> .
<http://www.ondex.org/bioknet/terms/Unit> <http://www.w3.org/1999/02/22-rdf-syntax-ns#type> <http://www.w3.org/2002/07/owl#Class> .
<http://www.ondex.org/bioknet/terms/Unit> <http://www.w3.org/2000/01/rdf-schema#label> "Unit"@en .
_:B77861368e8bb2f8d2dfef6b68718e585 <http://www.w3.org/2002/07/owl#onClass> <http://www.ondex.org/bioknet/terms/Unit> .
_:B77861368e8bb2f8d2dfef6b68718e585 <http://www.w3.org/2002/07/owl#onProperty> <http://www.ondex.org/bioknet/terms/attributeTypeUnit> .
_:B77861368e8bb2f8d2dfef6b68718e585 <http://www.w3.org/1999/02/22-rdf-syntax-ns#type> <http://www.w3.org/2002/07/owl#Restriction> .
_:B77861368e8bb2f8d2dfef6b68718e585 <http://www.w3.org/2002/07/owl#maxQualifiedCardinality> "1"^^<http://www.w3.org/2001/XMLSchema#nonNegativeInteger> .
<https://schema.org/rangeIncludes> <http://www.w3.org/1999/02/22-rdf-syntax-ns#type> <http://www.w3.org/2002/07/owl#AnnotationProperty> .
<http://www.ondex.org/bioknet/terms/Describeable> <http://www.w3.org/2004/02/skos/core#editorialNote> "[kNetMiner] these properties correspond to id, fullName, description in the ONDEX model."@en .
<http://www.ondex.org/bioknet/terms/Describeable> <http://www.w3.org/2000/01/rdf-schema#comment> "[editorial note] [kNetMiner] these properties correspond to id, fullName, description in the ONDEX model." .
<http://www.ondex.org/bioknet/terms/Describeable> <http://www.w3.org/2000/01/rdf-schema#comment> "[description] This is an abstract container to factorise those individuals for which a minimum of description attributes can be defined.\n\nThese are:\n\n- dcterms:identifier, to provide a resource identifier. Note that this is possibly valid only within a given context. it is also recommended that it is unique/unambiguous under that context, however, that is not strictly prescribed.\n\n- rdfs:label, to provide a resource human-readable label\n\n- dcterms:description, to provide a resource longer description." .
<http://www.ondex.org/bioknet/terms/Describeable> <http://www.w3.org/1999/02/22-rdf-syntax-ns#type> <http://www.w3.org/2002/07/owl#Class> .
<http://www.ondex.org/bioknet/terms/Describeable> <http://purl.org/dc/terms/description> "This is an abstract container to factorise those individuals for which a minimum of description attributes can be defined.\n\nThese are:\n\n- dcterms:identifier, to provide a resource identifier. Note that this is possibly valid only within a given context. it is also recommended that it is unique/unambiguous under that context, however, that is not strictly prescribed.\n\n- rdfs:label, to provide a resource human-readable label\n\n- dcterms:description, to provide a resource longer description."@en .
<http://www.ondex.org/bioknet/terms/Describeable> <http://www.w3.org/2000/01/rdf-schema#label> "Describeable Entity"@en .
_:Bec150e6e8653b51fcd8e13b7cab86016 <http://www.w3.org/2002/07/owl#unionOf> _:B69151a89349678f3f9ee83d0310425b8 .
_:Bec150e6e8653b51fcd8e13b7cab86016 <http://www.w3.org/1999/02/22-rdf-syntax-ns#type> <http://www.w3.org/2002/07/owl#Class> .
<http://www.ondex.org/bioknet/terms/Relation> <http://www.w3.org/2000/01/rdf-schema#comment> "[description] Relations in BioKNet are created in two ways:\n\n- as straight RDF statements between instances of Concept, and using subclasses of the relationType property.\n\n- as instances of Relation, with links from the Relation instance to the relation source (relFrom property), target (relTo property) and predicate (relTypeRef property). This way to define relations is well-known as reification and it is necessary when further properties/links need to be associated to a statement.\n\nThe main resource type that can be attached to a reified relation is bk:Attribute (bk:attribute property).\n\nWARNING: We strongly recommend that, if an instance of Relation (i.e., a reified relation) exists in a data set, then the corresponding plain triple exists too. For instance, if this is defined:\n\n<code>\nex:r0 a bk:Relation;\n  bk:relTypeRef ex:encodes;\n  bk:relFrom ex:gene0;\n  bk:relTo ex:prot0.\n</code>\n\nwe recommend to also define the triple ex:gene0 ex:encodes ex:prot0. This is to ease queries and start them from a base representation that is compliant with RDF principles.\n\nThe opposite (i.e., to create a bk:Relation for each bk:Concept triple based on subproperties of bk:relationType, even when there aren't further properties to attach to the triple) is less important, however, we recommend to introduce this redundancy, for the same sake of ease-to-write queries and performance.\n\nWe suggest to base the identifiers of reified relations on the IDs (or URIs) of its three parts, e.g., MD5 ( gene0 + encodes + prot0 ). This makes it easier to find the reified version of a relation once you have the components of its identifiers. WARNING: this should be considered an application facility and never be assumed as a reliable rule." .
<http://www.ondex.org/bioknet/terms/Relation> <http://www.w3.org/2000/01/rdf-schema#subClassOf> <http://www.ondex.org/bioknet/terms/RelationElement> .
<http://www.ondex.org/bioknet/terms/Relation> <http://www.w3.org/1999/02/22-rdf-syntax-ns#type> <http://www.w3.org/2002/07/owl#Class> .
<http://www.ondex.org/bioknet/terms/Relation> <http://purl.org/dc/terms/description> "Relations in BioKNet are created in two ways:\n\n- as straight RDF statements between instances of Concept, and using subclasses of the relationType property.\n\n- as instances of Relation, with links from the Relation instance to the relation source (relFrom property), target (relTo property) and predicate (relTypeRef property). This way to define relations is well-known as reification and it is necessary when further properties/links need to be associated to a statement.\n\nThe main resource type that can be attached to a reified relation is bk:Attribute (bk:attribute property).\n\nWARNING: We strongly recommend that, if an instance of Relation (i.e., a reified relation) exists in a data set, then the corresponding plain triple exists too. For instance, if this is defined:\n\n<code>\nex:r0 a bk:Relation;\n  bk:relTypeRef ex:encodes;\n  bk:relFrom ex:gene0;\n  bk:relTo ex:prot0.\n</code>\n\nwe recommend to also define the triple ex:gene0 ex:encodes ex:prot0. This is to ease queries and start them from a base representation that is compliant with RDF principles.\n\nThe opposite (i.e., to create a bk:Relation for each bk:Concept triple based on subproperties of bk:relationType, even when there aren't further properties to attach to the triple) is less important, however, we recommend to introduce this redundancy, for the same sake of ease-to-write queries and performance.\n\nWe suggest to base the identifiers of reified relations on the IDs (or URIs) of its three parts, e.g., MD5 ( gene0 + encodes + prot0 ). This makes it easier to find the reified version of a relation once you have the components of its identifiers. WARNING: this should be considered an application facility and never be assumed as a reliable rule."@en .
<http://www.ondex.org/bioknet/terms/Relation> <http://www.w3.org/2000/01/rdf-schema#label> "Relation"@en .
<http://purl.org/dc/terms/description> <http://www.w3.org/1999/02/22-rdf-syntax-ns#type> <http://www.w3.org/2002/07/owl#AnnotationProperty> .
<http://www.ondex.org/bioknet/terms/EvidenceType> <http://www.w3.org/2000/01/rdf-schema#subClassOf> <http://www.ondex.org/bioknet/terms/Describeable> .
<http://www.ondex.org/bioknet/terms/EvidenceType> <http://www.w3.org/1999/02/22-rdf-syntax-ns#type> <http://www.w3.org/2002/07/owl#Class> .
<http://www.ondex.org/bioknet/terms/EvidenceType> <http://www.w3.org/2000/01/rdf-schema#label> "Evidence Type"@en .
